# Snapshot report for `test/operators.js`

The actual snapshot is saved in `operators.js.snap`.

Generated by [AVA](https://avajs.dev).

## Force long operator with \`op` and \`` `op` ``]

> Snapshot 1

    '<math><mrow><mo>(</mo><mi /></mrow></math>'

> Snapshot 2

    '<math><mo>foo bar</mo><mo>`</mo></math>'

> Snapshot 3

    '<math><mo>(1)</mo></math>'

## Only force an operator when \ precedes a character

> Snapshot 1

    '<math><mo>\\</mo></math>'

## i hat

> Snapshot 1

    '<math><mover><mi>ı</mi><mo>^</mo></mover></math>'

## The operator (n) as an overscript

> Snapshot 1

    '<math><mover><mi>x</mi><mo>(n)</mo></mover></math>'

## Sums

> Snapshot 1

    '<math><munderover><mo>∑</mo><mrow><mi>n</mi><mo>=</mo><mn>0</mn></mrow><mi>k</mi></munderover><msub><mi>a</mi><mi>n</mi></msub><mo>=</mo><msub><mi>a</mi><mn>0</mn></msub><mo>+</mo><msub><mi>a</mi><mi>i</mi></msub><mo>+</mo><mo>⋯</mo><mo>+</mo><msub><mi>a</mi><mi>k</mi></msub></math>'

## Function composition

> Snapshot 1

    '<math><mi>𝐅</mi><mo>∘</mo><mi>𝐆</mi><mspace width="1ex" /><mo>:</mo><mspace width="1ex" /><mi>U</mi><mo>⊆</mo><msup><mi>ℝ</mi><mn>3</mn></msup><mo>→</mo><msup><mi>ℝ</mi><mn>2</mn></msup></math>'

## Eulers number

> Snapshot 1

    '<math><mi>e</mi><mo>=</mo><munderover><mo>∑</mo><mrow><mi>n</mi><mo>=</mo><mn>0</mn></mrow><mi>∞</mi></munderover><mfrac><mn>1</mn><mrow><mi>n</mi><mo>!</mo></mrow></mfrac></math>'

## Remove space around derivatives

> Snapshot 1

    '<math><mrow><mi>f</mi><mo lspace="0" rspace="0">′</mo><mrow><mo fence="true">(</mo><mi>x</mi><mo fence="true">)</mo></mrow></mrow></math>'

> Snapshot 2

    '<math><mrow><mi>f</mi><mo lspace="0" rspace="0">″</mo><mrow><mo fence="true">(</mo><mi>x</mi><mo fence="true">)</mo></mrow></mrow></math>'

> Snapshot 3

    '<math><mrow><mi>f</mi><mo lspace="0" rspace="0">‴</mo><mrow><mo fence="true">(</mo><mi>x</mi><mo fence="true">)</mo></mrow></mrow></math>'

> Snapshot 4

    '<math><mrow><mi>f</mi><mo lspace="0" rspace="0">⁗</mo><mrow><mo fence="true">(</mo><mi>x</mi><mo fence="true">)</mo></mrow></mrow></math>'

## Bayes theorem

> Snapshot 1

    '<math><mrow><mi>p</mi><mrow><mo fence="true">(</mo><mrow><mi>a</mi><mo>|</mo><mi>b</mi></mrow><mo fence="true">)</mo></mrow></mrow><mo>=</mo><mfrac><mrow><mi>p</mi><mrow><mo fence="true">(</mo><mrow><mi>b</mi><mo>|</mo><mi>a</mi></mrow><mo fence="true">)</mo></mrow><mi>p</mi><mrow><mo fence="true">(</mo><mi>a</mi><mo fence="true">)</mo></mrow></mrow><mrow><mi>p</mi><mrow><mo fence="true">(</mo><mi>b</mi><mo fence="true">)</mo></mrow></mrow></mfrac></math>'

## Gradient

> Snapshot 1

    '<math><mo>∇</mo><mrow><mi>f</mi><mrow><mo fence="true">(</mo><mrow><mi>x</mi><mo separator="true">,</mo><mi>y</mi></mrow><mo fence="true">)</mo></mrow></mrow><mo>=</mo><mrow><mo fence="true">(</mo><mrow><mrow><mfrac><mrow><mo>∂</mo><mi>f</mi></mrow><mrow><mo>∂</mo><mi>x</mi></mrow></mfrac><mrow><mo fence="true">(</mo><mrow><mi>x</mi><mo separator="true">,</mo><mi>y</mi></mrow><mo fence="true">)</mo></mrow></mrow><mo separator="true">,</mo><mrow><mfrac><mrow><mo>∂</mo><mi>f</mi></mrow><mrow><mo>∂</mo><mi>y</mi></mrow></mfrac><mrow><mo fence="true">(</mo><mrow><mi>x</mi><mo separator="true">,</mo><mi>y</mi></mrow><mo fence="true">)</mo></mrow></mrow></mrow><mo fence="true">)</mo></mrow></math>'

## Taylor polynomial

> Snapshot 1

    '<math><mrow><msub><mi>P</mi><mi>k</mi></msub><mrow><mo fence="true">(</mo><mi>x</mi><mo fence="true">)</mo></mrow></mrow><mo>=</mo><mrow><mi>f</mi><mrow><mo fence="true">(</mo><mi>a</mi><mo fence="true">)</mo></mrow></mrow><mo>+</mo><mrow><mi>f</mi><mo lspace="0" rspace="0">′</mo><mrow><mo fence="true">(</mo><mi>a</mi><mo fence="true">)</mo></mrow><mrow><mo fence="true">(</mo><mrow><mi>x</mi><mo>-</mo><mi>a</mi></mrow><mo fence="true">)</mo></mrow></mrow><mo>+</mo><mfrac><mrow><mi>f</mi><mo lspace="0" rspace="0">″</mo><mrow><mo fence="true">(</mo><mi>a</mi><mo fence="true">)</mo></mrow></mrow><mrow><mn>2</mn><mo>!</mo></mrow></mfrac><msup><mrow><mo fence="true">(</mo><mrow><mi>x</mi><mo>-</mo><mi>a</mi></mrow><mo fence="true">)</mo></mrow><mn>2</mn></msup><mo>+</mo><mo>⋯</mo><mo>+</mo><mfrac><mrow><msup><mi>f</mi><mrow><mo fence="true">(</mo><mi>k</mi><mo fence="true">)</mo></mrow></msup><mrow><mo fence="true">(</mo><mi>a</mi><mo fence="true">)</mo></mrow></mrow><mrow><mi>k</mi><mo>!</mo></mrow></mfrac><msup><mrow><mo fence="true">(</mo><mrow><mi>x</mi><mo>-</mo><mi>a</mi></mrow><mo fence="true">)</mo></mrow><mi>k</mi></msup></math>'

## Strokes theorem

> Snapshot 1

    '<math><msub><mo>∮</mo><mrow><mo>∂</mo><mi>S</mi></mrow></msub><mi>𝐅</mi><mo>·</mo><mi>d</mi><mi>𝐒</mi><mo>=</mo><msub><mo>∬</mo><mi>S</mi></msub><mo>∇</mo><mo>×</mo><mi>𝐅</mi><mo>·</mo><mi>d</mi><mi>𝐬</mi></math>'
